来源于 b 站 up PiKaChu345 8月22日发布的[每日一题](https://b23.tv/pmTwi1w)
### Question
> [! 问题 Question]  
> If $x_{n} \to x$ for $x \in \mathbb{R}$,  prove that
>
> $$ \lim_{ n \to \infty } \frac{{n \choose 0} x_{0} + {n \choose 1} x_{1} + \dots + {n \choose n} x_{n}}{2^{n}}  = x$$

### Solution
The following is my solution.

分段估计（Piecewise estimation)
Assume for $n > N_{\varepsilon} \in \mathbb{N}$,  $|x_{n} -x | < \frac{\varepsilon}{2}$,

Denote that for any $n \in \mathbb{N}$, 

$$ S_{n} := 2^{-n} \sum_{k=0}^{n} {n \choose k} |x_{n} - x| $$

So consider $S_{N_{\varepsilon}}$ as the first part, and $S_{n} - S_{N_{\varepsilon}}$ as the second part:
1. For the first part, use a lemma:
> [! Lemma]
> For any $m, n \in \mathbb{N}$, and $m \leq n$, the sequence
> 
> $$ y = {2n \choose m} $$
> 
> is increasing on $0 \leq m \leq n-1$.

And also since 

$$ 2^n = (1+1)^n = \sum_{k=0}^{n} {n \choose k} $$

 and 
 
 $${2n \choose m} = {2n \choose (2n-m)}$$
 
 , and denote $z^* = \max_{0 \leq m \leq N_{\varepsilon}} |x_{m}-x|$, it can be found that for 

$$ \forall n > N^* := \left\lceil \frac{2z^* N_{\varepsilon}}{\varepsilon}  \right\rceil ,$$

```math
\begin{equation}
\begin{aligned}
S_{N_{\varepsilon}} &= 2^{-n} \sum_{k=0}^{N_{\varepsilon}} {n \choose k} |x_{n} - x| \leq 2^{-n} z^* \sum_{k=0}^{N_{\varepsilon}} {n \choose k} \\ 
&\leq z^*  \frac{N_{\varepsilon}}{N^*} \leq z^* \frac{N_{\varepsilon} \varepsilon}{2z^* N_{\varepsilon}} = \frac{\varepsilon}{2}
\end{aligned}
\end{equation}
```

2. For the second part, for $n > N_{\varepsilon}$

```math
\begin{equation} \begin{aligned} S_{n} - S_{N_{\varepsilon}} &= 2^{-n} \sum_{k = N_{\varepsilon}+1}^{n} {n \choose k} |x_{k} -x| \leq 2^{-n} \sum_{k = N_{\varepsilon}+1}^{n} {n \choose k} \frac{\varepsilon}{2} \leq \frac{\varepsilon}{2}  \end{aligned} \end{equation}
```

Therefore, for $n > \max \{N^*, N_{\varepsilon}\}$, $S_{n} \to 0$ , so the original statement is proven.

### Proof of the Lemma
In the part of [Solution](#Solution), a lemma is used. The proof of the lemma is an induction:
1. **Base Step**: For $m=0$,
  
$$ {2n \choose 0} = 1 \leq 2n = {2n \choose 1} $$

2. **Induction Hypothesis**: 
	 Assume that for $m \leq n-2$, $\forall 0 \leq k \leq m$,

	 $$ {2n \choose k} \leq  {2n \choose m+1}$$

4. **Induction Step**:
	 For $m+1 < n-1$,
```math
\begin{equation}
\begin{aligned}
\frac{{2n \choose m+2}}{{2n \choose m+1}}  &= \frac{(2n)!}{(m+2)!\ (2n - m -2)!} \cdot \frac{(m+1)!\ (2n - m -1)!}{(2n)!} \\
&= \frac{2n-m-1}{m+2} \geq \frac{2n-n-1}{n} > 1
\end{aligned}
\end{equation}
```

### Toeplitz Theorem
[Reference](https://math.stackexchange.com/questions/2514778/toeplitz-theorem)
>[! Theorem]
>Let $a_{n}$ be a real sequence convergent to $a \in \mathbb{R}$. Let $c_{k, n}$ (where $1 \leq k \leq n$) be a sequence such that:
>```math
> \begin{equation} \tag{i}
> \begin{aligned}
> \forall k \lim_{ n \to \infty } c_{k,n} = 0
> \end{aligned}
> \end{equation} 
>```
>```math
> \begin{equation} \tag{ii}
> \begin{aligned}
> \lim_{ n \to \infty } \sum_{k=1}^n c_{k,n} = 1
> \end{aligned}
> \end{equation} 
>```
>```math
> \begin{equation} \tag{iii}
> \begin{aligned}
> \exists M > 0: \forall n, \quad \sum_{k=1}^n |c_{k,n}| \leq M
> \end{aligned}
> \end{equation} 
>```
> Then $\lim_{ n \to \infty } s_{n} = a$, where
>```math
> \begin{equation} \tag{iv}
> \begin{aligned}
> s_{n} \equiv \sum_{k=1}^n c_{k, n} \cdot a_{k}
> \end{aligned}
> \end{equation} 
>```

>[! Proof]
> If all the terms of the sequence $\{a_{n}\}$ are equal to $a$, then by $\mathrm{(ii)}$,
>
> $$ s_{n} = a \sum_{k=1}^n c_{k, n}, \quad \lim_{ n \to \infty } s_{n} = a \cdot 1 = a  $$
>
>  Thus it is enough to consider the case where the sequence converges to zero. 
>  Then, for any $m > 1$ and $n \geq m$,
>```math
> \begin{equation} \tag{*}
> \begin{aligned}
> |s_{n} - 0| &= \left| \sum_{k=1}^n c_{k, n} a_{k} \right| \\ 
> &\leq \sum_{k=1}^{m-1} |c_{k, n}| \cdot |a_{k}| + \sum_{k=m}^{n} |c_{k, n}| \cdot |a_{k}| 
> \end{aligned}
> \end{equation} 
>```
> The convergence to zero of $\{a_{n}\}$ implies that for a given $\varepsilon > 0$ there exists $n_{1}$ such that
>
> $$ |a_{n}| < \frac{\varepsilon}{2M} \quad \text{for} \quad n \geq n_{1} $$
>
> Of course, the sequence $\{a_{n}\}$ is bounded, say by $D > 0$. It follows from $\mathrm{(i)}$ that there exists $n_{2}$ such that for $n \geq n_{2}$, (because $n_{1}$ is a constant)
>
> $$\sum_{k=1}^{n_{1} -1} |c_{k,n}| < \frac{\varepsilon}{2D}.$$
>
> Next putting $m=n_{1}$ in $\mathrm{(*)}$, we get
>
> $$|s_{n}| \leq D \sum_{k=1}^{n_{1}-1} |c_{k, n}| + \frac{\varepsilon}{2M} \sum_{k=n_{1}}^{n} |c_{k, n}| < \frac{\varepsilon}{2} + \frac{\varepsilon}{2} = \varepsilon $$
>
> for  $n \geq \max\{n_{1}, n_{2}\}$. Hence $\lim_{ n \to \infty } s_{n} = 0$




